Refactor

Semantic/Stlc/BigStep/Denotation.lean
@@ -2,9 +2,6 @@ import Semantic.Stlc.TypeSystem
 import Semantic.Stlc.BigStep.Eval
 import Mathlib.Tactic
 
-inductive Exp.IsAbsVal : Exp n -> Prop where
-| abs : Exp.IsAbsVal (.abs T e)
-
 mutual
 
 def Ty.val_denot : Ty -> Exp 0 -> Prop
@@ -26,21 +23,10 @@ def Ty.exp_denot : Ty -> Exp 0 -> Prop
 
 end
 
-inductive Store : Nat -> Type where
-| nil : Store 0
-| cons : (e : Exp 0) -> (hv : e.IsVal) -> Store n -> Store (n + 1)
-
-def Store.lookup : Store n -> Var n -> Exp 0
-| .cons v _ s, .here => v
-| .cons _ _ s, .there i => s.lookup i
-
 def TypedStore : Store n -> Ctx n -> Prop
 | .nil, .empty => True
 | .cons v _ s, .var Γ T =>
   Ty.val_denot T v ∧ TypedStore s Γ
-
-def Subst.fromStore (s : Store n) : Subst n 0 where
-  exp := fun x => s.lookup x
 
 def SemanticTyping (Γ : Ctx n) (e : Exp n) (T : Ty) : Prop :=
   ∀ s,
@@ -48,24 +34,3 @@ def SemanticTyping (Γ : Ctx n) (e : Exp n) (T : Ty) : Prop :=
     Ty.exp_denot T (e.subst (Subst.fromStore s))
 
 notation:65 Γ " ⊨ " e " : " T => SemanticTyping Γ e T
-
-theorem Store.lookup_is_val {s : Store n} :
-  (s.lookup x).IsVal := by
-  induction x
-  case here => cases s; aesop
-  case there ih =>
-    cases s; simp [Store.lookup]
-    exact ih
-
-theorem Subst.fromStore_openVar_comp
-  (s : Store n) (v : Exp 0) (hv : v.IsVal) :
-  (Subst.fromStore s).liftVar.comp (Subst.openVar v) =
-    Subst.fromStore (Store.cons v hv s) := by
-  apply Subst.funext
-  intro x
-  cases x
-  case here => rfl
-  case there x0 =>
-    simp [Subst.comp, Subst.liftVar]
-    simp [Exp.openVar_succVar_comp]
-    rfl
